Modified AbstractMultiPaxosR3 to generate executable code

Isabelle2/AbstractMultiPaxosR3Correctness.thy
@@ -13,7 +13,7 @@ definition ref_map :: "('v,'a,'l)ampr2_state \<Rightarrow> ('v,'a,'l)amp_state" 
   "ref_map s \<equiv> \<lparr> amp_state.propCmd = (propCmd s),
   ballot = (\<lambda>a. ((ballot s) $ a)),
   vote = (\<lambda>a i b. (vote s $ a $ i $ b)),
-  suggestion = (\<lambda>i b. ((suggestion s i) $ b)),
+  suggestion = (\<lambda>i b. ((suggestion s $ i) $ b)),
   onebs = (\<lambda>a b. if (onebs s $ a $ b) = None then None else (Some (\<lambda>i. (the (onebs s $ a $ b)) $ i))),
   learned = (\<lambda>l i. (learned s $ l $ i)),
   leader = (\<lambda>a. (ampr2_state.leader s $ a)) \<rparr>"
@@ -24,7 +24,8 @@ term "ampr2_ioa"
 lemma aux_proof:"(op $ (K$ False)(leading b $:= True)) = (\<lambda> a . leading b = a)"
 proof
   fix a
-  have "(K$  False)(leading b $:= True) $ a = (leading b = a)"
+  let ?t = "(K$ False)(leading b $:= True) $ a = (leading b = a)"
+  have ?t
   proof(cases "leading b = a")
     case True
       thus ?thesis by (simp add: finfun_upd_apply_same)
@@ -32,69 +33,144 @@ proof
     case False
       thus ?thesis by (simp add: finfun_upd_apply)
   qed
-  thus "\<And>a. (K$  False)(leading b $:= True) $ a = (leading b = a)" by (simp add: finfun_upd_apply)
+  thus "\<And>a. ?t" by (simp add: finfun_upd_apply)
+qed
+ 
+subsection {* auxiliary lemmas for propose definition. *} 
+lemma aux_proof_propose:"\<And>c. (\<lambda>a b. if ampr2_state.onebs s $ a $ b = None then None
+  else Some (op $ (the (ampr2_state.onebs (s\<lparr>ampr2_state.propCmd := insert c (ampr2_state.propCmd s)\<rparr>) $ a $ b)))) = 
+    (\<lambda>a b. if ampr2_state.onebs s $ a $ b = None then None else Some (op $ (the (ampr2_state.onebs s $ a $ b))))"
+proof
+  fix c a
+  let ?t = "(\<lambda>b. if ampr2_state.onebs s $ a $ b = None then None
+    else Some (op $ (the (ampr2_state.onebs (s\<lparr>ampr2_state.propCmd := insert c (ampr2_state.propCmd s)\<rparr>) $ a $  b)))) =
+      (\<lambda>b. if ampr2_state.onebs s $ a $ b = None then None else Some (op $ (the (ampr2_state.onebs s $ a $ b))))"
+  have ?t
+  proof-
+    {
+      assume 0:"\<not>?t"
+      hence "False" by auto
+    }
+    thus ?t by blast
+  qed
+  thus "\<And>c a. ?t" by blast
 qed
 
-lemma aux_proof1:"\<And>l i v b q. \<lbrakk>q \<in> quorums; \<forall>a \<in> q. ampr2_state.vote s $ a $ i $ b = Some v\<rbrakk> \<Longrightarrow>
-    (\<lambda>la. op $ ((ampr2_state.learned s)(l $:= (ampr2_state.learned s $ l)(i $:= Some v)) $ la)) = 
-      (\<lambda>l. op $ (ampr2_state.learned s $ l))(l := op $ (ampr2_state.learned s $ l) (i \<mapsto> v))"
-proof
-  fix l i v b q la
-  assume 0:"q \<in> quorums" and 1:"\<forall>a \<in> q. ampr2_state.vote s $ a $ i $ b = Some v"
-  let ?t = "op $ ((ampr2_state.learned s)(l $:= (ampr2_state.learned  s $ l)(i $:= Some v)) $ la) =
-    ((\<lambda>l. op $ (ampr2_state.learned s $ l)) (l := op $ (ampr2_state.learned s $ l) (i \<mapsto> v))) la"
+subsection {* auxiliary lemmas for learn definition. *}
+
+lemma aux_proof_learn:"\<And>l i v. (\<lambda>a b. if ampr2_state.onebs s $ a $ b = None then None 
+  else Some (op $ (the (ampr2_state.onebs (s\<lparr>ampr2_state.learned := (ampr2_state.learned s)(l $:= (ampr2_state.learned s $ l)(i $:= Some v))\<rparr>) $ a $ b)))) 
+   = (\<lambda>a b.  if ampr2_state.onebs s $ a $ b = None then None else Some (op $ (the (ampr2_state.onebs s $ a $ b)))) 
+  \<and> (\<lambda>la. op $ ((ampr2_state.learned s)(l $:= (ampr2_state.learned s $ l)(i $:= Some v)) $ la)) =
+    (\<lambda>l. op $ (ampr2_state.learned s $ l))(l := op $ (ampr2_state.learned s $ l) (i \<mapsto> v))"
+proof-
+  fix l i v
+  let ?t1 = "(\<lambda>a b. if ampr2_state.onebs s $ a $ b = None then None 
+    else Some (op $ (the (ampr2_state.onebs (s\<lparr>ampr2_state.learned := (ampr2_state.learned s)(l $:= (ampr2_state.learned s $ l)(i $:= Some v))\<rparr>) $ a $ b)))) 
+    = (\<lambda>a b.  if ampr2_state.onebs s $ a $ b = None then None else Some (op $ (the (ampr2_state.onebs s $ a $ b))))"
+  let ?t2 = "(\<lambda>la. op $ ((ampr2_state.learned s)(l $:= (ampr2_state.learned s $ l)(i $:= Some v)) $ la)) =
+    (\<lambda>l. op $ (ampr2_state.learned s $ l))(l := op $ (ampr2_state.learned s $ l) (i \<mapsto> v))"
+  have 1:?t1
+  proof-
+    {
+      assume 0:"\<not>?t1"
+      hence "False" by force
+    }
+    thus ?t1 by blast
+  qed
+  have ?t2
+  proof-
+    {
+      assume 0:"\<not>?t2"
+      hence "False" by force
+    }
+    thus ?t2 by blast
+  qed
+  thus "\<And>l i v. ?t1 \<and> ?t2" using 1 by blast
+qed
+
+lemma aux_proof_learn1:"\<And>l i v. [b\<leftarrow>finfun_to_list (ampr2_state.suggestion s $ i) .
+  Set.filter (\<lambda>q. Set.filter (\<lambda>a. ampr2_state.vote s $ a $ i $ b = Some v) q = q) quorums \<noteq> {}] \<noteq> [] \<Longrightarrow>
+  \<exists>b q. q \<in> quorums \<and> (\<forall>a\<in>q. ampr2_state.vote s $ a $ i $ b = Some v)"
+proof-
+  fix l i v
+  let ?prems = "[b\<leftarrow>finfun_to_list (ampr2_state.suggestion s $ i) .
+    Set.filter (\<lambda>q. Set.filter (\<lambda>a. ampr2_state.vote s $ a $ i $ b = Some v) q = q) quorums \<noteq> {}] \<noteq> []"
+  let ?conc = "\<exists>b q. q \<in> quorums \<and> (\<forall>a\<in>q. ampr2_state.vote s $ a $ i $ b = Some v)"
+  assume 0:"[b\<leftarrow>finfun_to_list (ampr2_state.suggestion s $ i) .
+    Set.filter (\<lambda>q. Set.filter (\<lambda>a. ampr2_state.vote s $ a $ i $ b = Some v) q = q) quorums \<noteq> {}] \<noteq> []"
+  with this obtain b where 1:"Set.filter (\<lambda>q. Set.filter (\<lambda>a. ampr2_state.vote s $ a $ i $ b = Some v) q = q) quorums \<noteq> {}"
+    by (meson filter_False)
+  with this obtain q where 2:"q \<in> quorums" and 3:"Set.filter (\<lambda>a. ampr2_state.vote s $ a $ i $ b = Some v) q = q"
+    using Collect_empty_eq Set.filter_def by fastforce
+  hence "\<forall>a\<in>q. ampr2_state.vote s $ a $ i $ b = Some v" using member_filter by auto
+  thus "\<And>l i v. ?prems \<Longrightarrow> ?conc" using 0 2 by blast
+qed
+
+subsection {* auxiliary lemmas for join_ballot definition. *}
+lemma "acc_max voteimpl a b = distributed_safe_at.acc_max voteimpl a b"
+unfolding acc_max_def distributed_safe_at.acc_max_def sorry
+
+lemma aux_proof_join:"\<And>y xa. insts = (finfun_to_list (ampr2_state.vote s $ a)) \<Longrightarrow> 
+  fold (\<lambda>i ob. ob(i $:= acc_max (\<lambda>a. op $ (ampr2_state.vote s $ a $ i)) a b)) insts y $ xa =
+    distributed_safe_at.acc_max (\<lambda>a. op $ (ampr2_state.vote s $ a $ xa)) a b"
+proof-
+  fix y xa
+  assume 0:"insts = (finfun_to_list (ampr2_state.vote s $ a))"
+  let ?t = "fold (\<lambda>i ob. ob(i $:= acc_max (\<lambda>a. op $ (ampr2_state.vote s $ a $ i)) a b)) insts y $ xa =
+    distributed_safe_at.acc_max (\<lambda>a. op $ (ampr2_state.vote s $ a $ xa)) a b"
+  let ?t1 = "fold (\<lambda>i ob. ob(i $:= acc_max (\<lambda>a. op $ (ampr2_state.vote s $ a $ i)) a b)) insts y"
+  have "\<forall>i \<in> set insts. ?t1 $ i = acc_max (\<lambda>a. op $ (ampr2_state.vote s $ a $ i)) a b" sorry
   have ?t
-  proof(cases ?t)
+  proof(cases "xa \<in> set insts")
     case True
-      thus ?thesis by metis
+      thus ?thesis sorry
   next
     case False
-      thus ?thesis by (metis (no_types, lifting) finfun_update.rep_eq fun_upd_def)
+      hence "ampr2_state.vote s $ a $ xa = (K$ None)" using 0 sorry
+      thus ?thesis sorry
   qed
-  thus ?t by blast
+  thus "\<And>y xa. insts = (finfun_to_list (ampr2_state.vote s $ a)) \<Longrightarrow> ?t" by blast
 qed
 
-lemma aux_proof2:"\<lbrakk>b = ampr2_state.ballot s $ a; ampr2_state.suggestion s i $ b = None\<rbrakk> \<Longrightarrow>
-  (\<lambda>ia. op $ (if ia = i then (ampr2_state.suggestion s i)(b $:= Some v) else ampr2_state.suggestion s ia)) =
-    (\<lambda>i. op $ (ampr2_state.suggestion s i))(i := op $ (ampr2_state.suggestion s i) (b \<mapsto> v))"
-proof
-  fix ia
-  assume "b = ampr2_state.ballot s $ a" and "ampr2_state.suggestion s i $ b = None"
-  let ?t = "op $ (if ia = i then (ampr2_state.suggestion s i)(b $:= Some v) else ampr2_state.suggestion s ia) =
-    ((\<lambda>i. op $ (ampr2_state.suggestion s i))(i := op $ (ampr2_state.suggestion s i)(b \<mapsto> v))) ia"
-  have ?t
-  proof(cases ?t)
-    case True
-      thus ?thesis by metis
-  next
-    case False
-      thus ?thesis by (smt finfun_update.rep_eq fun_upd_apply)
-  qed
-  thus ?t by blast
-qed
-
-lemma aux_proof3:"(\<lambda>l. op $ ((ampr2_state.learned s)(l1 $:= (ampr2_state.learned s $ l1)(i $:= Some v)) $ l)) =
+subsection {* auxiliary lemmas for catch_up definition. *}
+lemma aux_proof_catchup:"(\<lambda>l. op $ ((ampr2_state.learned s)(l1 $:= (ampr2_state.learned s $ l1)(i $:= Some v)) $ l)) =
   (\<lambda>l. op $ (ampr2_state.learned s $ l))(l1 := op $ (ampr2_state.learned s $ l1)(i \<mapsto> v))"
 proof
   fix l
   let ?t = "op $ ((ampr2_state.learned s)(l1 $:= (ampr2_state.learned s $ l1)(i $:= Some v)) $ l) =
     ((\<lambda>l. op $ (ampr2_state.learned s $ l))(l1 := op $ (ampr2_state.learned s $ l1)(i \<mapsto> v))) l"
   have ?t
-  proof(cases ?t)
-    case True
-      thus ?thesis by blast
-  next
-    case False
-      thus ?thesis by auto
+  proof-
+    {
+      assume 0:"\<not>?t"
+      hence "False" by auto
+    }
+    thus ?t by blast
   qed
   thus "\<And>l. ?t" by blast
 qed
-  
-lemma aux_proof4:"\<And>c. (\<lambda>a b. if ampr2_state.onebs s $ a $ b = None then None
-  else Some (op $ (the (ampr2_state.onebs (s\<lparr>ampr2_state.propCmd := insert c (ampr2_state.propCmd s)\<rparr>) $ a $ b)))) = 
-    (\<lambda>a b. if ampr2_state.onebs s $ a $ b = None then None else Some (op $  (the (ampr2_state.onebs s $ a $  b))))"
-sorry
 
+lemma aux_proof_catchup1:"(\<lambda>a b. if ampr2_state.onebs s $ a $ b = None then None else 
+    Some (op $ (the (ampr2_state.onebs (s\<lparr>ampr2_state.learned := (ampr2_state.learned s)(l1 $:= (ampr2_state.learned s $ l1)(i $:= Some v))\<rparr>) $ a $ b)))) =
+    (\<lambda>a b. if ampr2_state.onebs s $ a $ b = None then None else Some (op $ (the (ampr2_state.onebs s $ a $ b))))"
+by (simp add: aux_proof_learn)
+
+subsection {* auxiliary lemmas for leadership definition. *}
+lemma aux_proof_leadership:"\<And>x. \<lbrakk>b = ampr2_state.ballot s $ aa; leading b = aa;
+  q \<in> quorums; \<not> ampr2_state.leader s $ aa;  \<forall>a\<in>q. \<exists>y. ampr2_state.onebs s $ a $ b = Some y\<rbrakk> \<Longrightarrow>
+  fold (\<lambda>i ss. ss(i $:= (ss $ i)(b $:= map_option fst (max_pair q (\<lambda>a. the (ampr2_state.onebs s $ a $ b) $ i)))))
+    (finfun_to_list (the (ampr2_state.onebs s $ aa $ b))) (ampr2_state.suggestion s) $ x $ b =
+  map_option fst (distributed_safe_at.max_pair q (\<lambda>a. the (if ampr2_state.onebs s $ a $ b = None
+    then None else Some (op $ (the (ampr2_state.onebs s $ a $ b)))) x))" sorry
+
+lemma aux_proof_leadership1:"\<And>x xa. \<lbrakk>b = ampr2_state.ballot s $ aa; leading b = aa; q \<in> quorums;
+  \<not> ampr2_state.leader s $ aa; \<forall>a\<in>q. \<exists>y. ampr2_state.onebs s $ a $ b = Some y; xa \<noteq> b\<rbrakk> \<Longrightarrow>
+  fold (\<lambda>i ss.  ss(i $:= (ss $ i)(b $:= map_option fst (max_pair q (\<lambda>a. the (ampr2_state.onebs s $ a $ b) $ i)))))
+    (finfun_to_list (the (ampr2_state.onebs s $ aa $ b))) (ampr2_state.suggestion s) $ x $ xa =
+  ampr2_state.suggestion s $ x $ xa" sorry
+
+subsection {* lemma for refinement relationship between ampr1_ioa and ampr2_ioa. *}
 lemma "is_ref_map ref_map ampr2_ioa ampr1_ioa"
 proof (auto simp add:is_ref_map_def simp del:split_paired_Ex)
   fix s
@@ -112,16 +188,17 @@ next
     apply (simp add:ampr1_ioa_def ampr1.amp_ioa_def ampr1.amp_trans_def)
     apply (induct rule:trans_cases_2)
     (* propose *)
-    apply (simp add:simps ampr1.simps ref_map_def aux_proof4)
+    apply (simp add:simps ampr1.simps ref_map_def aux_proof_propose)
     (* learn *)
     apply (simp add:simps ampr1.simps ref_map_def ballot_array.chosen_def ballot_array.chosen_at_def)
-    
+    apply (simp add:aux_proof_learn aux_proof_learn1)
     (* join_ballot *)
     apply (induct a) apply auto[2]
     subgoal premises prems for a b
     proof -
       have "ampr1.join_ballot a b (ref_map s) (ref_map t)" using prems
-        by (auto simp add:ref_map_def simps Let_def ampr1.simps fun_eq_iff)
+        apply (auto simp add:join_ballot_def ampr1.join_ballot_def ref_map_def)
+        by (auto simp add:ref_map_def simps Let_def ampr1.simps fun_eq_iff aux_proof_join)
       thus ?thesis by auto
     qed
     (* do_vote *)
@@ -129,7 +206,7 @@ next
     subgoal premises prems for a i v
     proof -
       have "ampr1.do_vote a i v (ref_map s) (ref_map t)" using prems
-        by (auto simp add:ref_map_def simps Let_def ampr1.simps fun_eq_iff)
+        by (auto simp add:ref_map_def simps Let_def ampr1.simps fun_eq_iff )
       thus ?thesis by auto
     qed
     (* suggest *)
@@ -137,7 +214,8 @@ next
     subgoal premises prems for a i b v
     proof -
       have "ampr1.suggest a i b v (ref_map s) (ref_map t)" using prems(1)
-        by (auto simp add:suggest_def ampr1.suggest_def ref_map_def aux_proof2)
+        apply (auto simp add:suggest_def ampr1.suggest_def ref_map_def) 
+        by (auto simp add:simps Let_def ampr1.simps fun_eq_iff)
       thus ?thesis by auto
     qed
     (* catch_up *)
@@ -145,7 +223,7 @@ next
     subgoal premises prems for l1 l2 i v
     proof -
       have "ampr1.catch_up l1 l2 i v (ref_map s) (ref_map t)" using prems
-        by (auto simp add:catch_up_def ampr1.catch_up_def ref_map_def aux_proof3)
+        by (auto simp add:catch_up_def ampr1.catch_up_def ref_map_def aux_proof_catchup aux_proof_catchup1)
       thus ?thesis by auto
     qed
     (* acquire_leadership *)
@@ -154,7 +232,9 @@ next
     proof -
       have "ampr1.acquire_leadership aa q (ref_map s) (ref_map t)" using prems
         apply (auto simp add:acquire_leadership_def ampr1.acquire_leadership_def ref_map_def)
-        by (auto simp add:simps Let_def ampr1.simps fun_eq_iff)
+        apply (auto simp add:simps Let_def ampr1.simps fun_eq_iff)
+        apply (simp add:aux_proof_leadership)
+        using aux_proof_leadership1 by blast
       thus ?thesis by auto
     qed
     done 
